Exploration for LRU cache

Test/tutorial/LRU_cache/three.dfy
@@ -2,97 +2,38 @@ datatype Outcome<T> =
 	| Success(value: T)
 	| Failure
 
-datatype entry<T> = Entry(key: nat,value: T)
+datatype entry<T(!new,==)> = Entry(key: nat,value: T)
 	
-// trait Storage<T(!new,==)> {
-
-// 	ghost var log: seq<entry<T>>
-
-// 	function last_occurence_pre(key: nat, log': seq<entry<T>>): Outcome<T> {
-// 		var size: nat := |log'|;
-// 		if size == 0 then
-// 			Failure
-// 		else
-// 			var candidate: entry := log'[size-1];
-// 			if candidate.key == key then
-// 				Success(candidate.value)
-// 			else
-// 				last_occurence_pre(key, log'[..(size-1)])
-// 	}
-
-// 	function last_occurence(key: nat): Outcome<T>
-// 		reads this
-// 	{
-// 		last_occurence_pre(key,log)
-// 	}
-	
-// 	predicate Invariant()
-// 		reads this
-
-// 	method get(key: nat) returns (result: Outcome<T>)
-// 		requires Invariant()
-// 		ensures Invariant()
-// 		ensures result.Success? <==> exists index: nat :: index < |log| && log[index].key == key 
-// 		ensures result.Success? ==> last_occurence(key).Success? && last_occurence(key).value == result.value
-		
-// 	function method fget(key: nat): Outcome<T>
-//  		reads this
-// 		requires Invariant()
-		
-// 	method put(key: nat, value: T)
-// 	 	modifies this
-// 		requires Invariant()
-// 		ensures log == old(log) + [Entry(key,value)]
-// 		ensures Invariant()
-		
-// }
-
 datatype Option<T> =
 	| Some(value: T)
 	| None
 
-class Item<T> {
-
+class Item<T(!new,==)> {
+	
 	var more_recently_used: Option<Item<T>>
 	var less_recently_used: Option<Item<T>>
 	const key: nat
-	const value: T
+	var value: T
 
-		
-	constructor(key: nat, value: T) {
+	constructor(key: nat, value: T)
+		ensures this.key == key
+		ensures this.value == value
+		ensures this.more_recently_used == None
+		ensures this.less_recently_used == None
+	{
 
 		this.key := key;
 		this.value := value;
 		more_recently_used := None;
 		less_recently_used := None;
-		
+
 	}
 	
 }
 
-class MapStorage<T(!new,==)> {
+class LRUCache<T(!new,==)> {
 
 	ghost var Repr: set<Item<T>>;
-
-	ghost var log: seq<entry<T>>
-
-	function last_occurence_pre(key: nat, log': seq<entry<T>>): Outcome<T> {
-		var size: nat := |log'|;
-		if size == 0 then
-			Failure
-		else
-			var candidate: entry := log'[size-1];
-			if candidate.key == key then
-				Success(candidate.value)
-			else
-				last_occurence_pre(key, log'[..(size-1)])
-	}
-
-	function last_occurence(key: nat): Outcome<T>
-		reads this
-	{
-		last_occurence_pre(key,log)
-	}
 	
 	var storage: map<nat,T>
 
@@ -100,142 +41,177 @@ class MapStorage<T(!new,==)> {
 		
 	var cache_head: Option<Item<T>>
 	var cache_tail: Option<Item<T>>
-	var cache_map: map<nat,Item<T>>
+	var cache: map<nat,Item<T>>
 
 	predicate Invariant()
 		reads this, Repr
 	{
-		&& (forall key: nat :: key in storage <==> exists index: nat :: index < |log| && log[index].key == key)
-		&& (forall key: nat :: forall value: T :: (key in storage && storage[key] == value) ==> last_occurence(key).Success? && last_occurence(key).value == value)
-		&& (forall key: nat :: key in cache_map ==> cache_map[key] in Repr)
+		&& (forall key: nat :: key in cache ==> key in storage)
+		&& (forall key: nat :: key in cache ==> cache[key] in Repr)
+		&& (forall key: nat :: key in cache ==> cache[key].key == key)
+		&& (forall key: nat :: key in cache ==> cache[key].value == storage[key])
 		&& (cache_head.Some? ==> cache_head.value in Repr)
 		&& (cache_tail.Some? ==> cache_tail.value in Repr)
-		&& (forall i: Item :: i in Repr && i.more_recently_used.Some? ==> i.more_recently_used.value in Repr)
-		&& (forall i: Item :: i in Repr && i.less_recently_used.Some? ==> i.less_recently_used.value in Repr)
+		&& (forall i: Item :: i in Repr ==> i.more_recently_used.None? || i.more_recently_used.value in Repr)
+		&& (forall i: Item :: i in Repr ==> i.less_recently_used.None? || i.less_recently_used.value in Repr)
+		&& (forall key, key': nat :: key in cache && key' in cache && key != key' ==> cache[key] != cache[key'])
+		&& (cache_head.Some? ==> cache_head.value.more_recently_used.None?)
+		&& (cache_tail.Some? ==> cache_tail.value.less_recently_used.None?)
+		&& (forall i: Item :: i in Repr && Some(i) != cache_head ==> i.more_recently_used.Some?)
+		&& (forall i: Item :: i in Repr && Some(i) != cache_tail ==> i.less_recently_used.Some?)
+		&& (forall i: Item :: i in Repr && i.more_recently_used.Some? ==> i.more_recently_used.value.less_recently_used == Some(i))
+		&& (forall i: Item :: i in Repr && i.less_recently_used.Some? ==> i.less_recently_used.value.more_recently_used == Some(i))
+		&& (|cache| == 0 ==> cache_head == cache_tail == None)
+		&& (|cache| == 1 ==> cache_head == cache_tail)
+		&& (|cache| >= 1 ==> cache_head.Some? && cache_tail.Some?)
+		&& (|cache| >= 2 <==> cache_head != cache_tail)
+
 	}
 	
 	constructor(size: nat)
+		requires size >= 2
 		ensures Invariant()
 	{
 		cache_size := size;
 		storage := map[];
-		log := [];
 		cache_head := None;
 		cache_tail := None;
-		cache_map := map[];
+		cache := map[];
 		Repr := {};
 	}
 
-	method promote(item: Item)
-		requires Invariant()
-		ensures Invariant()
-
-	method evict()
-		requires Invariant()
+	method promote(key: nat)
 		modifies this, Repr
+		requires key in cache
+		requires Invariant()
 		ensures Invariant()
+		//ensures cache_head.Some? ==> cache_head.value.key == key
 	{
-		if |cache_map| == cache_size {
-			if cache_tail.None? {
-				// Cannot happen
-			} else {
-				if cache_tail.value.more_recently_used.None? {
-					// Cannot happen
+		var item := cache[key];
+		if |cache| >= 2 {
+			if item.more_recently_used.Some? {
+				if item.less_recently_used.Some? {
+					assert cache_tail.value.less_recently_used.None?;
+					item.more_recently_used.value.less_recently_used := item.less_recently_used;
+					//assert cache_tail.value.less_recently_used.None?;
+					item.less_recently_used.value.more_recently_used := item.more_recently_used;
+					cache_head.value.less_recently_used := Some(item);
+					item.less_recently_used := cache_head;
+					item.more_recently_used := None;
+					cache_head := Some(item);
+					//assume false;
 				} else {
-					var previous_item: Option<Item> := cache_tail.value.more_recently_used;
-					if previous_item.None? {
-						// Cannot happen 
-					} else {
-						previous_item.value.less_recently_used := None;
-						cache_map := cache_map - {previous_item.value.key};
-						Repr := Repr - {previous_item.value};
-						cache_tail := previous_item;
-						assume false;
-					}
+					
+					//assert |cache| >= 2 ==> cache_head != cache_tail;
+					cache_tail := item.more_recently_used;
+					cache_tail.value.less_recently_used := None;
+					//item.more_recently_used.value.less_recently_used := None;
+					cache_head.value.less_recently_used := Some(item);
+					var old_cache_head := cache_head;
+					cache_head := Some(item);
+					cache_head.value.less_recently_used := old_cache_head;
+					cache_head.value.more_recently_used := None;
+					assume false;
 				}
 			}
-		}	
+		}
 	}
-
-	method introduce(key: nat, value: T)
+	
+	method put_cache(key: nat, value: T)
+		modifies this, Repr
+		requires key in storage   // Very convenient because this is known from the calling context
+		requires storage[key] == value
+		requires key !in cache
 		requires Invariant()
-		modifies this
 		ensures Invariant()
 	{
+
 		var item: Item := new Item(key,value);
-		item.less_recently_used := cache_head;
-		cache_map := cache_map[key := item];
-		cache_head := Some(item);
 		Repr := Repr + {item};
-		assume false;
+		
+		if |cache| == 0 {
+			cache := cache[key := item];
+			cache_head := Some(item);
+			cache_tail := Some(item);
+		} else {
+			item.less_recently_used := cache_head;
+			cache := cache[key := item];
+			cache_head.value.more_recently_used := Some(item);
+			cache_head := Some(item);
+		}
+		
+		//assume false;
+
+		// Will do eviction later
+		
+		// if |cache| == cache_size {
+		// 	if cache_tail.None? {
+		// 		// Cannot happen
+		// 	} else {
+		// 		if cache_tail.value.more_recently_used.None? {
+		// 			// Cannot happen
+		// 		} else {
+		// 			var previous_item: Option<Item> := cache_tail.value.more_recently_used;
+		// 			if previous_item.None? {
+		// 				// Cannot happen 
+		// 			} else {
+		// 				previous_item.value.less_recently_used := None;
+		// 				cache := cache - {previous_item.value.key};
+		// 				Repr := Repr - {previous_item.value};
+		// 				cache_tail := previous_item;
+		// 			}
+		// 		}
+		// 	}
+		// }
+
+			
+		
 	}
 	
 	method get(key: nat) returns (result: Outcome<T>)
 		modifies this, Repr
 		requires Invariant()
 		ensures Invariant()
-		ensures result.Success? <==> exists index: nat :: index < |log| && log[index].key == key
-		ensures result.Success? ==> last_occurence(key).Success? && last_occurence(key).value == result.value
 	{
-		if key in cache_map {
-			result := Success(cache_map[key].value);
-			promote(cache_map[key]);
-			assume false;
+		if key in cache {
+			result := Success(cache[key].value);
+			promote(key);
 		} else if key in storage {
 			var value: T := storage[key];
 			result := Success(value);
-			evict();
-			introduce(key,value);
-			assume false;
+			put_cache(key,value);
 		} else {
 			result := Failure;
 		}
 	}
 
 	method put(key: nat, value: T)
-		modifies this
+		modifies this, Repr
 		requires Invariant()
-		ensures log == old(log) + [Entry(key,value)]
 		ensures Invariant()
 	{
-
-		assert forall key: nat :: key in storage <==> exists index: nat :: index < |log| && log[index].key == key;
+		//assert forall key': nat :: key' in cache ==> cache[key'].value == storage[key'];
 
 		storage := storage[key := value];
 
-		assert forall key: nat :: key in old(storage) <==> exists index: nat :: index < |log| && log[index].key == key;
+		//assert forall key': nat :: key' in cache && key' != key ==> cache[key'].value == storage[key'];
+		//assert forall key': nat :: key' in cache ==> cache[key'].value == old(storage)[key'];
 
-		log := log + [Entry(key,value)];
-
-		assert forall key: nat :: key in old(storage) <==> exists index: nat :: index < |old(log)| && old(log)[index].key == key;
-
-		forall key': nat ensures key' in storage ==> exists index: nat :: index < |log| && log[index].key == key' {
-			if key' in storage {
-				if key == key' {
-					var index: nat := |log| - 1;
-					assert log[index].key == key;
-				} else {
-					assert key' in old(storage);
-					var index: nat :| index < |old(log)| && old(log)[index].key == key';
-					assert log[index].key == old(log)[index].key;
-				}
-			}
+		if key in cache {
+			cache[key].value := value;
+			assert cache[key].value == storage[key];
+			// assert forall key': nat :: key' != key && key' in cache ==> cache[key'].value == storage[key'] by {
+			// 	forall key': nat ensures key' != key && key' in cache ==> cache[key'].value == storage[key'] {
+			// 		if key' != key && key' in cache {
+			// 			assert cache[key'].value == old(cache)[key'].value;
+			// 			assert storage[key'] == old(storage)[key'];
+			// 			// Aliasing!
+			// 			assert old(cache)[key'].value == old(cache[key'].value);
+			// 			assert old(cache[key'].value) == old(storage)[key'];
+			// 		}
+			// 	}
+			// }
 		}
-	}
-
-	function method fget(key: nat): Outcome<T>
-		reads this, Repr
-		requires Invariant()
-	{
-		if key in storage then Success(storage[key]) else Failure
-	}
-	
-	lemma prop_test_1(key: nat)
-		requires Invariant()
-		requires fget(key).Success?
-		ensures exists index: nat :: index < |log| && log[index].key == key
-		ensures last_occurence(key).Success? && last_occurence(key).value == fget(key).value
-	{
 	}
 
 }
